Read optimized reference

src/examples/read_optimized_reference.v
@@ -35,8 +35,7 @@ Definition RR_write : expr :=
     "per" <-_NA "v" ;;
     Flush "per" ;;
     FenceSync ;;
-    "vol" <-_NA "v" ;;
-    #().
+    "vol" <-_NA "v".
 
 Definition RR_recover : expr :=
   λ: "rr",
@@ -60,39 +59,43 @@ Section spec.
   Qed.
 
   Definition is_RR (vrr : val) v : dProp Σ :=
-    ∃ (ℓp ℓv : loc) ss n,
-      "%lastEq" ∷ ⌜ last ss = Some (mk_numbered n v) ⌝ ∗
+    ∃ (ℓp ℓv : loc) n ss,
       "->" ∷ ⌜ vrr = (#ℓp, #ℓv)%V ⌝ ∗
-      "pPts" ∷ ℓp ↦_{rr_prot} ss ∗
+      "pPts" ∷ ℓp ↦_{rr_prot} [mk_numbered n v] ∗
       "perLb" ∷ persist_lb ℓp rr_prot (mk_numbered n v) ∗
-      "vPts" ∷ ℓv ↦_{rr_prot} ss.
+      "vPts" ∷ ℓv ↦_{rr_prot} (ss ++ [mk_numbered n v]).
 
   Definition is_recoverable_RR (vrr : val) v : dProp Σ :=
-    ∃ (ℓp ℓv : loc) ss n,
-      ⌜ last ss = Some (mk_numbered n v) ⌝ ∗
-      ⌜ vrr = (#ℓp, #ℓv)%V ⌝ ∗
-      ℓp ↦_{rr_prot} ss ∗ persist_lb ℓp rr_prot (mk_numbered n v).
+    ∃ (ℓp ℓv : loc) n,
+      "->" ∷ ⌜ vrr = (#ℓp, #ℓv)%V ⌝ ∗
+      "pPts" ∷ ℓp ↦_{rr_prot} [mk_numbered n v] ∗
+      "perLb" ∷ persist_lb ℓp rr_prot (mk_numbered n v).
+
+  Lemma crash_condition_impl' n v ℓp (ℓv : loc) :
+    ℓp ↦_{rr_prot} [mk_numbered n v] -∗
+    persist_lb ℓp rr_prot (mk_numbered n v) -∗
+    <PC> is_recoverable_RR (#ℓp, #ℓv) v.
+  Proof.
+    iIntros "pPts perLb".
+    iModIntro.
+    iDestruct "perLb" as "(per & Hh)".
+    iDestruct "Hh" as (sRec incl) "#crashedIn".
+    iDestruct (crashed_in_if_rec with "crashedIn pPts")
+      as (??) "(%prefix & crashedIn2 & pPts)".
+    apply prefix_app_singleton in prefix as [-> ->].
+    simpl.
+    iExists ℓp, ℓv, n.
+    iSplitPure; first done.
+    simpl.
+    iFrame "pPts".
+    iFrame "per".
+  Qed.
 
   Lemma is_RR_post_crash vrr v :
     is_RR vrr v ⊢ <PC> is_recoverable_RR vrr v.
   Proof.
-    iDestruct 1 as (ℓp ℓv ss n) "(%lastEq & vrrEq & pPts & flushLb & isRR)".
-    iDestruct (mapsto_na_increasing_list with "pPts") as %incr.
-    apply last_Some in lastEq as (ss', ->).
-    iModIntro.
-    iDestruct "flushLb" as "(per & Hh)".
-    iDestruct "Hh" as (sRec incl) "#crashedIn".
-    iDestruct (crashed_in_if_rec with "crashedIn pPts")
-      as (??) "(%prefix & crashedIn2 & pPts)".
-    iDestruct (crashed_in_agree with "crashedIn crashedIn2") as %<-.
-    assert (sRec = (mk_numbered n v)) as ->.
-    { apply (anti_symm (⊑@{numbered val})); last done.
-      apply: prefix_increasing_list_snoc; try done. }
-    simpl.
-    iExists ℓp, ℓv, _, n.
-    iSplitPure; first apply last_snoc.
-    iFrame "vrrEq pPts".
-    iFrame "per".
+    iNamed 1.
+    iApply (crash_condition_impl' with "pPts perLb").
   Qed.
 
   Lemma RR_init_spec (v : val) s E :
@@ -112,22 +115,69 @@ Section spec.
     wp_apply (wp_alloc_na v (mk_numbered 0 v) rr_prot); simpl; first done.
     iIntros (ℓv) "vPts".
     wp_pures.
-    iModIntro. repeat iExists _. iFrame "pPts vPts perLb". done.
+    iModIntro. iExists _, _, _, [].
+    iSplitPure; first done. iFrameF "pPts". iFrame "vPts perLb".
   Qed.
 
-  Lemma crash_condition_impl n v ss ℓp ℓv :
-    ⌜ last ss = Some (mk_numbered n v) ⌝ -∗
-    ℓp ↦_{rr_prot} ss -∗
+  Lemma crash_condition_impl n v ℓp (ℓv : loc) :
+    ℓp ↦_{rr_prot} [mk_numbered n v] -∗
+    ℓv ↦_{rr_prot} [mk_numbered n v] -∗
     persist_lb ℓp rr_prot (mk_numbered n v) -∗
-    ℓv ↦_{rr_prot} ss -∗
     <PC> is_recoverable_RR (#ℓp, #ℓv) v.
   Proof.
-    iIntros (?) "pPts perLb vPts".
+    iIntros "pPts vPts perLb".
     iApply is_RR_post_crash.
-    repeat iExists _.
-    iSplitPure; first eassumption.
-    iSplitPure; first reflexivity.
+    iExists ℓp, ℓv, n, [].
+    iSplitPure; first done.
     iFrame.
+  Qed.
+
+  Lemma prefix_of_2 {A} (xs : list A) x1 x2 :
+    xs `prefix_of` [x1; x2] →
+    xs = [] ∨ xs = [x1] ∨ xs = [x1; x2].
+  Proof.
+    destruct xs as [|x1' xs]. { naive_solver. }
+    intros [-> pre]%prefix_cons_inv.
+    destruct xs as [|x2' xs]. { naive_solver. }
+    apply prefix_cons_inv in pre as [-> pre].
+    apply prefix_nil_inv in pre as ->.
+    naive_solver.
+  Qed.
+
+  Lemma crash_condition_impl_2 n v w ℓp (ℓv : loc) :
+    ℓp ↦_{rr_prot} [mk_numbered n v; mk_numbered (n + 1) w] -∗
+    persist_lb ℓp rr_prot (mk_numbered n v) -∗
+    <PC> ∃ u, is_recoverable_RR (#ℓp, #ℓv) u ∗ ⌜ u = v ∨ u = w ⌝.
+  Proof.
+    iIntros "pPts perLb".
+    iCrashIntro.
+    iDestruct "perLb" as "[per (% & hi & crashedIn)]".
+    iDestruct (crashed_in_if_rec with "crashedIn pPts")
+      as (??) "(%pre & crashedIn2 & pPts)".
+    apply prefix_of_2 in pre as [eq | [eq | eq]].
+    { destruct ss'; inversion eq. }
+    - destruct ss'; inversion eq.
+      2: { destruct ss'; inversion eq. }
+      iExists v.
+      iSplit; last naive_solver.
+      repeat iExists _.
+      iSplitPure; first done.
+      iFrameF "pPts".
+      simpl.
+      iFrame "per".
+    - destruct ss'; inversion eq.
+      destruct ss'; inversion eq.
+      2: { simpl in eq. destruct ss'; inversion eq. }
+      iExists w.
+      iSplit; last naive_solver.
+      iExists _, _, (n + 1).
+      iSplitPure; first done.
+      iDestruct (crashed_in_persist_lb with "crashedIn2") as "#per2".
+      simpl.
+      iFrame "per2".
+      iDestruct (mapsto_na_persist_lb with "pPts per2") as "HII".
+      { intros [?|?]; lia. }
+      iFrame "HII".
   Qed.
 
   Lemma RR_read_spec rv (v : val) s E :
@@ -138,17 +188,18 @@ Section spec.
     iNamed 1.
     rewrite /RR_read.
     wpc_pures.
-    { iApply (crash_condition_impl with "[//] pPts perLb vPts"). }
+    { iApply (crash_condition_impl' with "pPts perLb"). }
     iApply wpc_atomic_no_mask.
     iSplit.
-    { iApply (crash_condition_impl with "[//] pPts perLb vPts"). }
-    wp_apply (wp_load_na with "[$vPts]"); first eassumption.
+    { iApply (crash_condition_impl' with "pPts perLb"). }
+    wp_apply (wp_load_na with "[$vPts]").
+    { apply last_snoc. }
     { iModIntro. simpl.
       iIntros (?) "#H". iFrame "H". rewrite right_id. iApply "H". }
     iIntros (?) "(vPts & <-)".
     iSplit.
     { iModIntro.
-      iApply (crash_condition_impl with "[//] pPts perLb vPts"). }
+      iApply (crash_condition_impl' with "pPts perLb"). }
     iModIntro. iSplitPure; first reflexivity.
     repeat iExists _.
     iFrame "pPts vPts perLb".
@@ -157,14 +208,127 @@ Section spec.
 
   Lemma RR_write_spec rv (v w : val) s E :
     is_RR rv v -∗
-    WPC RR_write rv w @ s; E {{ _, is_RR rv w }} {{ True }}%I.
+    WPC RR_write rv w @ s; E
+      {{ _, is_RR rv w }}
+      {{ <PC> ∃ u, is_recoverable_RR rv u ∗ ⌜ u = v ∨ u = w ⌝}}%I.
   Proof.
-  Admitted.
+    iNamed 1.
+    rewrite /RR_write.
+    wpc_pures.
+    { iApply post_crash_mono;
+        last iApply (crash_condition_impl' with "pPts perLb").
+      iIntros "H". iExists _. iFrame "H". naive_solver. }
+
+    wpc_bind (_ <-_NA _)%E.
+    iApply wpc_atomic_no_mask.
+    iSplit.
+    { iApply post_crash_mono;
+        last iApply (crash_condition_impl' with "pPts perLb").
+      iIntros "H". iExists _. iFrame "H". naive_solver. }
+    iApply (wp_store_na _ rr_prot _ _ _ (mk_numbered (n + 1) w) with "[$pPts]").
+    { done. }
+    { apply numbered_le. lia. }
+    { simpl. done. }
+    iIntros "!> pPts".
+    iSplit.
+    { iApply (crash_condition_impl_2 with "pPts perLb"). }
+    iModIntro.
+    wpc_pures.
+    { iApply (crash_condition_impl_2 with "pPts perLb"). }
+
+    wpc_bind (Flush _)%E.
+    iApply wpc_atomic_no_mask.
+    iSplit.
+    { iApply (crash_condition_impl_2 with "pPts perLb"). }
+    iApply (wp_flush_na with "pPts").
+    iNext.
+    iIntros "(pPts & ? & pLb)".
+    iSplit.
+    { iModIntro. iApply (crash_condition_impl_2 with "pPts perLb"). }
+    iModIntro.
+    wpc_pures.
+    { iApply (crash_condition_impl_2 with "pPts perLb"). }
+
+    (* The fence. *)
+    wpc_bind (FenceSync)%E.
+    iApply wpc_atomic_no_mask.
+    iSplit. { iApply (crash_condition_impl_2 with "pPts perLb"). }
+    iApply wp_fence_sync. do 2 iModIntro.
+    iSplit. { iApply (crash_condition_impl_2 with "pPts perLb"). }
+    iModIntro.
+    iDestruct "pLb" as "#pLb".
+    wpc_pures.
+    { iApply (crash_condition_impl_2 with "pPts perLb"). }
+
+    iDestruct (mapsto_na_persist_lb with "pPts pLb") as "pPts".
+    { intros [?|?]; lia. }
+
+    iApply wpc_atomic_no_mask.
+    iSplit. {
+      iApply post_crash_mono;
+        last iApply (crash_condition_impl' with "pPts pLb").
+      iIntros "H". iExists _. iFrame "H". naive_solver. }
+
+    iApply (wp_store_na _ rr_prot _ _ _ (mk_numbered (n + 1) w) with "[$vPts]").
+    { apply last_snoc. }
+    { apply numbered_le. lia. }
+    { simpl. done. }
+    iIntros "!> vPts".
+    iSplit. {
+      iApply post_crash_mono;
+        last iApply (crash_condition_impl' with "pPts pLb").
+      iIntros "H". iExists _. iFrame "H". naive_solver. }
+    iModIntro.
+    repeat iExists _.
+    iSplitPure; first done.
+    iFrameF "pPts".
+    iFrameF "pLb".
+    iFrame "vPts".
+  Qed.
 
   Lemma RR_recover_spec rv (v w : val) s E :
     is_recoverable_RR rv v -∗
-    WPC RR_recover rv @ s; E {{ rv2, is_RR rv2 v }} {{ True }}%I.
+    WPC RR_recover rv @ s; E
+      {{ rv2, is_RR rv2 v }}
+      {{ <PC> is_recoverable_RR rv v }}%I.
   Proof.
-  Admitted.
+    iNamed 1.
+    rewrite /RR_recover.
+    wpc_pures.
+    { iApply (crash_condition_impl' with "pPts perLb"). }
+
+    wpc_bind (!_NA _)%E.
+    iApply wpc_atomic_no_mask.
+    iSplit.
+    { iApply (crash_condition_impl' with "pPts perLb"). }
+    wp_apply (wp_load_na with "[$pPts]").
+    { done. }
+    { iModIntro. simpl.
+      iIntros (?) "#H". iFrame "H". rewrite right_id. iApply "H". }
+    iIntros (?) "(pPts & <-)".
+    iSplit.
+    { iModIntro.
+      iApply (crash_condition_impl' with "pPts perLb"). }
+    iModIntro.
+
+    wpc_bind (ref_NA _)%E.
+    iApply wpc_atomic_no_mask.
+    iSplit. { iApply (crash_condition_impl' with "pPts perLb"). }
+    wp_apply (wp_alloc_na v (mk_numbered n v) rr_prot); simpl; first done.
+    iIntros (ℓv') "vPts".
+    iSplit.
+    { iModIntro.
+      iApply (crash_condition_impl' with "pPts perLb"). }
+    iModIntro.
+
+    wpc_pures.
+    { iApply (crash_condition_impl' with "pPts perLb"). }
+    iModIntro.
+    iExists _, _, _, [].
+    iSplitPure; first done.
+    iFrameF "pPts".
+    iFrameF "perLb".
+    iFrame "vPts".
+  Qed.
 
 End spec.
